Progress on segment theorem

theories/contextual_refinement.v
@@ -1,7 +1,7 @@
 From stdpp Require Import gmap fin_maps fin_sets.
 
 From cap_machine Require Import machine_parameters cap_lang.
-From cap_machine Require Import stdpp_img linking machine_run.
+From cap_machine Require Import stdpp_img linking machine_run addr_reg_sample.
 
 (** Minimal free memory in which to write our contexts *)
 Definition reserved_context_size_z: Z := 100000.
@@ -54,6 +54,66 @@ Section contextual_refinement.
     contextual_refinement impl spec.
 
   Infix "≼ᵣ" := contextual_refinement (at level 80).
+
+  (** A simple function generating dummy export (all 0)
+      for a given list of imports, usefull for building contexts *)
+  Section dummy_exports.
+    Definition dummy_exports target : exports_type Symbols :=
+      map_fold (fun _ s exp => <[s:=WInt 0]> exp)
+      ∅ target.(imports).
+
+    Lemma dummy_exports_spec target : forall s,
+      match dummy_exports target !! s with
+        | None => s ∉ img target.(imports)
+        | Some w => w = WInt 0 /\ s ∈ img target.(imports)
+      end.
+    Proof.
+      apply (map_fold_ind
+        (fun m imp => ∀ k, match m !! k with
+          | None => k ∉ img imp
+          | Some w => w = WInt 0 /\ k ∈ img imp
+        end)
+        (fun (_:Addr) (s:Symbols) exp => <[s:=WInt 0]> exp)).
+      intros s. rewrite lookup_empty. rewrite img_empty_L. set_solver.
+      intros a s exp exp' imp IH k.
+      destruct (Symbols_eq_dec s k) as [sk | sk].
+      rewrite sk. rewrite lookup_insert.
+      split. reflexivity. rewrite elem_of_img. exists a. apply lookup_insert.
+      rewrite lookup_insert_ne. 2: exact sk.
+      specialize (IH k). destruct (exp' !! k).
+      destruct IH as [IHw Hexp].
+      split. exact IHw.
+      rewrite elem_of_img. rewrite elem_of_img in Hexp. destruct Hexp as [a' Hexp].
+      exists a'. rewrite lookup_insert_ne. exact Hexp.
+      intros aa'. rewrite aa' in imp. rewrite imp in Hexp. discriminate.
+      rewrite elem_of_img. rewrite elem_of_img in IH.
+      intros [a' Hexp].
+      apply lookup_insert_Some in Hexp.
+      destruct Hexp as [ [aa' ss'] | [aa' Hexpa'] ].
+      contradiction.
+      apply (IH (ex_intro _ _ Hexpa')).
+    Qed.
+    Lemma dummy_exports_lookup {target} :
+      ∀ w, w ∈ img (dummy_exports target) -> w = WInt 0.
+    Proof.
+      intros w Hsw. apply elem_of_img in Hsw. destruct Hsw as [s Hsw].
+      specialize (dummy_exports_spec target s). intros H.
+      rewrite Hsw in H. destruct H. exact H.
+    Qed.
+    Lemma dummy_exports_from_imports {target} :
+      dom (dummy_exports target) = img (target.(imports)).
+    Proof.
+      apply set_eq.
+      intros s.
+      specialize (dummy_exports_spec target s). intros H.
+      rewrite elem_of_dom.
+      split. intros [w Hde_s_w]. rewrite Hde_s_w in H. destruct H. exact H0.
+      intros Himg.
+      destruct (Some_dec (dummy_exports target !! s)) as [ [w Hexp_s] | Hexp_s];
+      rewrite Hexp_s; rewrite Hexp_s in H. auto.
+      contradiction.
+    Qed.
+  End dummy_exports.
 
   Section facts.
     Lemma ctxt_ref_reflexive {comp}:
@@ -114,8 +174,7 @@ Section contextual_refinement.
       2,3,4: solve_can_link.
       transitivity (resolve_imports (imports (ctxt ⋈ spec)) (exports extra) (segment (ctxt ⋈ spec))).
       rewrite Hexp.
-      pose (@resolve_imports_exports_empty Symbols _ _) as ri.
-      unfold exports_type in ri. rewrite ri. reflexivity.
+      rewrite resolve_imports_exports_empty. reflexivity.
       apply map_union_subseteq_l.
       inversion Hc.
 
@@ -130,17 +189,17 @@ Section contextual_refinement.
 
       assert (Hex: ∀ w, w ∈ img (exports ctxt ∪ exports spec) -> can_address_only w (dom (segment (ctxt ⋈ spec)))).
       intros w Hw'. apply elem_of_img in Hw' as [s Hw'].
-      apply lookup_union_Some_raw in Hw' as [Hw' | [_ Hw']].
+      apply lookup_union_Some_raw in Hw' as [Hw' | [_ Hw'] ].
       apply (can_address_only_subseteq_stable2 w (dom (segment ctxt)) _ Hdom_ctxt).
-      inversion ctxt_impl as [[[]]]. apply Hwr_exp. apply elem_of_img_rev in Hw'. assumption.
+      inversion ctxt_impl as [ [ [] ] ]. apply Hwr_exp. apply elem_of_img_rev in Hw'. assumption.
       apply (can_address_only_subseteq_stable2 w (dom (segment spec)) _ Hdom_spec).
       inversion Hcan_link. inversion Hwf_r. apply Hwr_exp. apply elem_of_img_rev in Hw'. assumption.
 
       assert (Hse: ∀ a' w, (segment ctxt ∪ segment spec) !! a' = Some w -> can_address_only w (dom (segment (ctxt ⋈ spec)))).
       intros a w Hw'.
-      apply lookup_union_Some_raw in Hw' as [Hw' | [_ Hw']].
+      apply lookup_union_Some_raw in Hw' as [Hw' | [_ Hw'] ].
       apply (can_address_only_subseteq_stable2 w (dom (segment ctxt)) _ Hdom_ctxt).
-      inversion ctxt_impl as [[[]]]. apply Hwr_ms. apply elem_of_img_rev in Hw'. assumption.
+      inversion ctxt_impl as [ [ [] ] ]. apply Hwr_ms. apply elem_of_img_rev in Hw'. assumption.
       apply (can_address_only_subseteq_stable2 w (dom (segment spec)) _ Hdom_spec).
       inversion Hcan_link. inversion Hwf_r. apply Hwr_ms. apply elem_of_img_rev in Hw'. assumption.
 
@@ -149,23 +208,165 @@ Section contextual_refinement.
       unfold link in Hw. simpl in Hw.
       rewrite resolve_imports_spec in Hw.
       destruct (imports spec !! a).
-      destruct ((exports ctxt ∪ exports spec) !! s) eqn:He;
-      unfold exports_type in Hw; rewrite He in Hw. apply Some_inj in Hw. rewrite <-Hw.
+      destruct ((exports ctxt ∪ exports spec) !! s) eqn:He.
+      apply Some_inj in Hw. rewrite <-Hw.
       apply elem_of_img_rev in He. apply (Hex _ He).
       1,2: rewrite resolve_imports_spec in Hw;
            destruct (imports ctxt !! a) as [s'|]; apply (Hse _ _ Hw) ||
            destruct ((exports ctxt ∪ exports spec) !! s') eqn:He';
-           unfold exports_type in Hw; rewrite He' in Hw;
            apply (Hse _ _ Hw) || apply Some_inj in Hw; rewrite <-Hw;
            apply elem_of_img_rev in He'; apply (Hex _ He').
-
 
       inversion ctxt_impl. intros w Hw.
       apply (can_address_only_subseteq_stable2 w (dom (segment ctxt)) _ Hdom_ctxt).
       apply (Hwr_regs w Hw).
-
       Unshelve. solve_can_link.
     Qed.
+
+    (* When a ≼ᵣ b then
+       - dom (imports b) ⊆ dom (imports a)
+       - dom (segment b) ⊆ dom (segment a) *)
+    Section component_part_subseteq.
+      (** Basic context to prove the forall is non-empty
+          Halt immediatly *)
+      Example halt_context addr target : component Symbols := {|
+        segment := {[ addr := halt ]};
+        imports := ∅;
+        exports := dummy_exports target;
+      |}.
+
+      Lemma halt_context_wf {addr target}:
+        well_formed_comp can_address_only unconstrained_addr (halt_context addr target).
+      Proof.
+        unfold halt_context.
+        apply wf_comp_intro; simpl.
+        - rewrite img_empty_L. apply disjoint_empty_r.
+        - rewrite dom_empty. apply empty_subseteq.
+        - intros w exp_s.
+          apply dummy_exports_lookup in exp_s.
+          rewrite exp_s. unfold can_address_only. exact I.
+        - intros w H. apply img_singleton, elem_of_singleton in H.
+          rewrite H. exact I.
+        - exact I.
+      Qed.
+
+      Lemma halt_context_can_link {addr target} :
+        wf_comp target -> addr ∉ dom (segment target) ->
+        can_link can_address_only unconstrained_addr (halt_context addr target) target.
+      Proof.
+        intros t_wf Haddr.
+        apply can_link_intro.
+        - apply halt_context_wf.
+        - apply (wf_comp_weaken_ar any_implies_unconstrained_addr t_wf).
+        - rewrite map_disjoint_spec. intros i x y Hix Hiy.
+          apply Haddr.
+          unfold halt_context in Hix. simpl in Hix.
+          apply lookup_singleton_Some in Hix as [Hi _].
+          rewrite -Hi in Hiy. apply mk_is_Some, elem_of_dom in Hiy. apply Hiy.
+        - inversion t_wf.
+          rewrite map_disjoint_dom.
+          rewrite dummy_exports_from_imports.
+          symmetry. exact Hdisj.
+      Qed.
+
+      Lemma halt_context_machine_run {addr target} :
+        wf_comp target -> addr ∉ dom (segment target) -> (addr <? addr ^+ 1 = true)%a ->
+        machine_run 2 (Executable, (
+          {[ PC := WCap RWX addr (addr^+1)%a addr ]},
+          segment ((halt_context addr target) ⋈ target))
+        ) = Some Halted.
+      Proof.
+        intros wft Haddr Haddr'.
+        unfold machine_run.
+        rewrite lookup_singleton.
+        unfold isCorrectPCb.
+        replace ((addr <=? addr)%a && (addr <? addr ^+ 1)%a && (isPerm RWX RX || isPerm RWX RWX)) with true.
+        simpl.
+        rewrite resolve_imports_spec.
+        replace (imports target !! addr) with (@None Symbols).
+        rewrite resolve_imports_spec lookup_empty.
+        replace (({[addr := halt]} ∪ segment target) !! addr) with (Some halt).
+        unfold exec, exec_opt, halt; rewrite (decode_encode_instrW_inv Halt); simpl.
+        reflexivity.
+        symmetry. apply lookup_union_Some_l. apply lookup_singleton.
+        destruct (imports target !! addr) as [w|] eqn:Hita.
+        exfalso. apply Haddr.
+        inversion wft. apply Himp. apply mk_is_Some, elem_of_dom in Hita. apply Hita.
+        reflexivity.
+        simpl. symmetry. rewrite andb_true_iff. split.
+        rewrite andb_true_iff. split. solve_finz. solve_addr. reflexivity.
+        (* specialize (Har_ms addr (Himp addr Hita)).
+        unfold finz.lt in Har_ms.
+        rewrite reserved_context_size_to_z in Har_ms.
+        simpl in Har_ms. unfold reserved_context_size_z in Har_ms.
+        lia. reflexivity. *)
+      Qed.
+
+      Lemma halt_context_is_context {addr target} :
+        wf_comp target -> addr ∉ dom (segment target) ->
+        is_context can_address_only unconstrained_addr
+          (halt_context addr target) target {[ PC := WCap RWX addr (addr^+1)%a addr ]}.
+      Proof.
+        intros Hwf_t Haddr.
+        apply is_context_intro.
+        - apply (halt_context_can_link Hwf_t Haddr).
+        - intros w Hsr_w.
+          apply img_singleton, elem_of_singleton in Hsr_w.
+          rewrite Hsr_w.
+          intros a Ha01. simpl. rewrite dom_singleton elem_of_singleton.
+          solve_finz.
+        - rewrite dummy_exports_from_imports. reflexivity.
+        - simpl. rewrite img_empty_L. apply empty_subseteq.
+      Qed.
+
+      (** Contextual refinement implies that the
+          implementation imports all the specifications symbols *)
+      Lemma ctxt_ref_imports_subseteq {impl spec: component Symbols}:
+        contextual_refinement impl spec ->
+        img spec.(imports) ⊆ img impl.(imports).
+      Proof.
+        intros Href s Hspec_s.
+        inversion Href.
+        assert (H: 0%a ∉ (dom (segment impl))).
+        { intros Hita. inversion Hwf_impl.
+          specialize (Har_ms 0%a Hita). solve_finz. }
+        assert (H1 : (0 <? 0 ^+ 1 = true)%a). auto.
+        specialize (Hrefines
+          (halt_context 0%a impl)
+          {[ PC := WCap RWX za (za^+1)%a za ]} _
+          (halt_context_is_context Hwf_impl H)
+          (ex_intro _ 2 (halt_context_machine_run Hwf_impl H H1))).
+        destruct Hrefines as [Hctxt_spec _].
+        inversion Hctxt_spec.
+        specialize (Hno_imps_l s Hspec_s).
+        simpl in Hno_imps_l.
+        rewrite dummy_exports_from_imports in Hno_imps_l.
+        apply Hno_imps_l.
+      Qed.
+
+      Lemma ctxt_ref_segment_subseteq {impl spec}:
+        impl ≼ᵣ spec ->
+        dom spec.(segment) ⊆ dom impl.(segment).
+      Proof.
+        intros [ ] a Ha.
+        destruct (segment impl !! a) as [w|] eqn:HeqA.
+        apply mk_is_Some, elem_of_dom in HeqA. apply HeqA.
+        apply not_elem_of_dom in HeqA.
+        assert (H1 : (a <? a ^+ 1 = true)%a). admit.
+        specialize (Hrefines
+          (halt_context a impl)
+          {[ PC := WCap RWX a (a^+1)%a a ]} _
+          (halt_context_is_context Hwf_impl HeqA)
+          (ex_intro _ 2 (halt_context_machine_run Hwf_impl HeqA H1))).
+        destruct Hrefines as [Hctxt_spec _].
+        inversion Hctxt_spec. inversion Hcan_link.
+        rewrite map_disjoint_dom in Hms_disj.
+        exfalso. apply (Hms_disj a).
+        unfold halt_context. simpl. rewrite dom_singleton elem_of_singleton.
+        reflexivity.
+        assumption.
+      Admitted.
+    End component_part_subseteq.
 
     (* Lemma ctxt_ref_segment_subseteq {impl spec}:
       impl ≼ᵣ spec ->
